include/s2n-bignum-c89.h
@@ -49,6 +49,10 @@ extern void bignum_add_p384 (uint64_t z[6], uint64_t x[6], uint64_t y[6]);
 /*  Inputs x[9], y[9]; output z[9] */
 extern void bignum_add_p521 (uint64_t z[9], uint64_t x[9], uint64_t y[9]);
 
+/*  Add modulo p_sm2, z := (x + y) mod p_sm2, assuming x and y reduced */
+/*  Inputs x[4], y[4]; output z[4] */
+extern void bignum_add_sm2 (uint64_t z[4], uint64_t x[4], uint64_t y[4]);
+
 /*  Compute "amontification" constant z :== 2^{128k} (congruent mod m) */
 /*  Input m[k]; output z[k]; temporary buffer t[>=k] */
 extern void bignum_amontifier (uint64_t k, uint64_t *z, uint64_t *m, uint64_t *t);
@@ -670,6 +674,10 @@ extern void bignum_sub_p384 (uint64_t z[6], uint64_t x[6], uint64_t y[6]);
 /*  Subtract modulo p_521, z := (x - y) mod p_521, assuming x and y reduced */
 /*  Inputs x[9], y[9]; output z[9] */
 extern void bignum_sub_p521 (uint64_t z[9], uint64_t x[9], uint64_t y[9]);
+
+/*  Subtract modulo p_sm2, z := (x - y) mod p_sm2, assuming x and y reduced */
+/*  Inputs x[4], y[4]; output z[4] */
+extern void bignum_sub_sm2 (uint64_t z[4], uint64_t x[4], uint64_t y[4]);
 
 /*  Convert 4-digit (256-bit) bignum to big-endian bytes */
 /*  Input x[4]; output z[32] (bytes) */
