tests/test.c
@@ -252,6 +252,28 @@ uint64_t k_25519[4] =
    UINT64_C(0x2406d9dc56dffce7)
  };
 
+// Parameters for sm2
+
+uint64_t p_sm2[4] =
+ { UINT64_C(0xFFFFFFFFFFFFFFFF),
+   UINT64_C(0xFFFFFFFF00000000),
+   UINT64_C(0xFFFFFFFFFFFFFFFF),
+   UINT64_C(0xFFFFFFFEFFFFFFFF)
+};
+
+uint64_t n_sm2[4] =
+ { UINT64_C(0x53BBF40939D54123),
+   UINT64_C(0x7203DF6B21C6052B),
+   UINT64_C(0xFFFFFFFFFFFFFFFF),
+   UINT64_C(0xFFFFFFFEFFFFFFFF)
+};
+
+uint64_t i_sm2[4] =
+ { UINT64_C(0x0000000000000001),
+   UINT64_C(0xFFFFFFFF00000001),
+   UINT64_C(0xFFFFFFFE00000000),
+   UINT64_C(0xFFFFFFFC00000001)
+ };
 
 // ****************************************************************************
 // Reference implementations, basic and stupid ones in C
@@ -1368,6 +1390,42 @@ int test_bignum_add_p521(void)
                     "...0x%016"PRIx64" + ...0x%016"PRIx64" mod ....0x%016"PRIx64" = "
                     "...0x%016"PRIx64"\n",
                     k,b0[0],b1[0],p_521[0],b2[0]);
+      }
+   }
+  printf("All OK\n");
+  return 0;
+}
+
+int test_bignum_add_sm2(void)
+{ uint64_t i, k;
+  printf("Testing bignum_add_sm2 with %d cases\n",tests);
+  uint64_t c;
+  for (i = 0; i < tests; ++i)
+   { k = 4;
+     random_bignum(k,b2); reference_mod(k,b0,b2,p_sm2);
+     random_bignum(k,b2); reference_mod(k,b1,b2,p_sm2);
+     bignum_add_sm2(b2,b0,b1);
+     reference_copy(k+1,b3,k,b0);
+     reference_copy(k+1,b4,k,b1);
+     reference_add_samelen(k+1,b4,b4,b3);
+     reference_copy(k+1,b3,k,p_sm2);
+     reference_mod(k+1,b5,b4,b3);
+     reference_copy(k,b3,k+1,b5);
+
+     c = reference_compare(k,b3,k,b2);
+     if (c != 0)
+      { printf("### Disparity: [size %4"PRIu64"] "
+               "...0x%016"PRIx64" + ...0x%016"PRIx64" mod ....0x%016"PRIx64" = "
+               "...0x%016"PRIx64" not ...0x%016"PRIx64"\n",
+               k,b0[0],b1[0],p_sm2[0],b2[0],b3[0]);
+        return 1;
+      }
+     else if (VERBOSE)
+      { if (k == 0) printf("OK: [size %4"PRIu64"]\n",k);
+        else printf("OK: [size %4"PRIu64"] "
+                    "...0x%016"PRIx64" + ...0x%016"PRIx64" mod ....0x%016"PRIx64" = "
+                    "...0x%016"PRIx64"\n",
+                    k,b0[0],b1[0],p_sm2[0],b2[0]);
       }
    }
   printf("All OK\n");
@@ -6924,6 +6982,43 @@ int test_bignum_sub_p521(void)
   return 0;
 }
 
+int test_bignum_sub_sm2(void)
+{ uint64_t i, k;
+  printf("Testing bignum_sub_sm2 with %d cases\n",tests);
+  uint64_t c;
+  for (i = 0; i < tests; ++i)
+   { k = 4;
+     random_bignum(k,b2); reference_mod(k,b0,b2,p_sm2);
+     random_bignum(k,b2); reference_mod(k,b1,b2,p_sm2);
+     bignum_sub_sm2(b2,b0,b1);
+     reference_copy(k+1,b3,k,p_sm2);
+     reference_copy(k+1,b4,k,b0);
+     reference_copy(k+1,b5,k,b1);
+     reference_add_samelen(k+1,b4,b4,b3);
+     reference_sub_samelen(k+1,b4,b4,b5);
+     reference_mod(k+1,b5,b4,b3);
+     reference_copy(k,b3,k+1,b5);
+
+     c = reference_compare(k,b3,k,b2);
+     if (c != 0)
+      { printf("### Disparity: [size %4"PRIu64"] "
+               "...0x%016"PRIx64" - ...0x%016"PRIx64" mod ....0x%016"PRIx64" = "
+               "...0x%016"PRIx64" not ...0x%016"PRIx64"\n",
+               k,b0[0],b1[0],p_sm2[0],b2[0],b3[0]);
+        return 1;
+      }
+     else if (VERBOSE)
+      { if (k == 0) printf("OK: [size %4"PRIu64"]\n",k);
+        else printf("OK: [size %4"PRIu64"] "
+                    "...0x%016"PRIx64" - ...0x%016"PRIx64" mod ....0x%016"PRIx64" = "
+                    "...0x%016"PRIx64"\n",
+                    k,b0[0],b1[0],p_sm2[0],b2[0]);
+      }
+   }
+  printf("All OK\n");
+  return 0;
+}
+
 int test_bignum_tobebytes_4(void)
 { uint64_t t;
   printf("Testing bignum_tobebytes_4 with %d cases\n",tests);
@@ -9027,6 +9122,7 @@ int main(int argc, char *argv[])
   functionaltest(all,"bignum_add_p256k1",test_bignum_add_p256k1);
   functionaltest(all,"bignum_add_p384",test_bignum_add_p384);
   functionaltest(all,"bignum_add_p521",test_bignum_add_p521);
+  functionaltest(all,"bignum_add_sm2",test_bignum_add_sm2);
   functionaltest(all,"bignum_amontifier",test_bignum_amontifier);
   functionaltest(all,"bignum_amontmul",test_bignum_amontmul);
   functionaltest(all,"bignum_amontredc",test_bignum_amontredc);
@@ -9208,6 +9304,7 @@ int main(int argc, char *argv[])
   functionaltest(all,"bignum_sub_p256k1",test_bignum_sub_p256k1);
   functionaltest(all,"bignum_sub_p384",test_bignum_sub_p384);
   functionaltest(all,"bignum_sub_p521",test_bignum_sub_p521);
+  functionaltest(all,"bignum_sub_sm2",test_bignum_sub_sm2);
   functionaltest(all,"bignum_tobebytes_4",test_bignum_tobebytes_4);
   functionaltest(all,"bignum_tobebytes_6",test_bignum_tobebytes_6);
   functionaltest(all,"bignum_tolebytes_4",test_bignum_tolebytes_4);
