arm/proofs/bignum_add_sm2.ml
@@ -4,13 +4,13 @@
  *)
 
 (* ========================================================================= *)
-(* Addition modulo p_256, the field characteristic for the NIST P-256 curve. *)
+(* Addition modulo p_sm2, the field characteristic for the CC SM2 curve.     *)
 (* ========================================================================= *)
 
-(**** print_literal_from_elf "arm/p256/bignum_add_p256.o";;
+(**** print_literal_from_elf "arm/sm2/bignum_add_sm2.o";;
  ****)
 
-let bignum_add_p256_mc = define_assert_from_elf "bignum_add_p256_mc" "arm/p256/bignum_add_p256.o"
+let bignum_add_sm2_mc = define_assert_from_elf "bignum_add_sm2_mc" "arm/sm2/bignum_add_sm2.o"
 [
   0xa9401424;       (* arm_LDP X4 X5 X1 (Immediate_Offset (iword (&0))) *)
   0xa9402448;       (* arm_LDP X8 X9 X2 (Immediate_Offset (iword (&0))) *)
@@ -22,10 +22,10 @@ let bignum_add_p256_mc = define_assert_from_elf "bignum_add_p256_mc" "arm/p256/b
   0xba0b00e7;       (* arm_ADCS X7 X7 X11 *)
   0x9a1f03e3;       (* arm_ADC X3 XZR XZR *)
   0xb1000488;       (* arm_ADDS X8 X4 (rvalue (word 1)) *)
-  0xb2407fe9;       (* arm_MOV X9 (rvalue (word 4294967295)) *)
+  0xb2607fe9;       (* arm_MOV X9 (rvalue (word 18446744069414584320)) *)
   0xfa0900a9;       (* arm_SBCS X9 X5 X9 *)
-  0xfa1f00ca;       (* arm_SBCS X10 X6 XZR *)
-  0xb26083eb;       (* arm_MOV X11 (rvalue (word 18446744069414584321)) *)
+  0xba1f00ca;       (* arm_ADCS X10 X6 XZR *)
+  0x92c0002b;       (* arm_MOVN X11 (word 1) 32 *)
   0xfa0b00eb;       (* arm_SBCS X11 X7 X11 *)
   0xfa1f0063;       (* arm_SBCS X3 X3 XZR *)
   0x9a883084;       (* arm_CSEL X4 X4 X8 Condition_CC *)
@@ -37,26 +37,26 @@ let bignum_add_p256_mc = define_assert_from_elf "bignum_add_p256_mc" "arm/p256/b
   0xd65f03c0        (* arm_RET X30 *)
 ];;
 
-let BIGNUM_ADD_P256_EXEC = ARM_MK_EXEC_RULE bignum_add_p256_mc;;
+let BIGNUM_ADD_SM2_EXEC = ARM_MK_EXEC_RULE bignum_add_sm2_mc;;
 
 (* ------------------------------------------------------------------------- *)
 (* Proof.                                                                    *)
 (* ------------------------------------------------------------------------- *)
 
-let p_256 = new_definition `p_256 = 115792089210356248762697446949407573530086143415290314195533631308867097853951`;;
+let p_sm2 = new_definition `p_sm2 = 0xFFFFFFFEFFFFFFFFFFFFFFFFFFFFFFFFFFFFFFFF00000000FFFFFFFFFFFFFFFF`;;
 
-let BIGNUM_ADD_P256_CORRECT = time prove
+let BIGNUM_ADD_SM2_CORRECT = time prove
  (`!z x y m n pc.
         nonoverlapping (word pc,0x5c) (z,8 * 4)
         ==> ensures arm
-             (\s. aligned_bytes_loaded s (word pc) bignum_add_p256_mc /\
+             (\s. aligned_bytes_loaded s (word pc) bignum_add_sm2_mc /\
                   read PC s = word pc /\
                   C_ARGUMENTS [z; x; y] s /\
                   bignum_from_memory (x,4) s = m /\
                   bignum_from_memory (y,4) s = n)
              (\s. read PC s = word (pc + 0x58) /\
-                  (m < p_256 /\ n < p_256
-                   ==> bignum_from_memory (z,4) s = (m + n) MOD p_256))
+                  (m < p_sm2 /\ n < p_sm2
+                   ==> bignum_from_memory (z,4) s = (m + n) MOD p_sm2))
           (MAYCHANGE [PC; X3; X4; X5; X6; X7; X8; X9; X10; X11] ,,
            MAYCHANGE SOME_FLAGS ,,
            MAYCHANGE [memory :> bignum(z,4)])`,
@@ -67,7 +67,7 @@ let BIGNUM_ADD_P256_CORRECT = time prove
   REWRITE_TAC[BIGNUM_FROM_MEMORY_BYTES] THEN ENSURES_INIT_TAC "s0" THEN
   BIGNUM_DIGITIZE_TAC "m_" `read (memory :> bytes (x,8 * 4)) s0` THEN
   BIGNUM_DIGITIZE_TAC "n_" `read (memory :> bytes (y,8 * 4)) s0` THEN
-  ARM_ACCSTEPS_TAC BIGNUM_ADD_P256_EXEC
+  ARM_ACCSTEPS_TAC BIGNUM_ADD_SM2_EXEC
    [3;4;7;8;10;12;13;15;16] (1--22) THEN
   ENSURES_FINAL_STATE_TAC THEN ASM_REWRITE_TAC[] THEN STRIP_TAC THEN
   RULE_ASSUM_TAC(REWRITE_RULE
@@ -76,20 +76,20 @@ let BIGNUM_ADD_P256_CORRECT = time prove
   ASM_REWRITE_TAC[] THEN DISCARD_STATE_TAC "s22" THEN
   MATCH_MP_TAC EQUAL_FROM_CONGRUENT_MOD_MOD THEN MAP_EVERY EXISTS_TAC
    [`64 * 4`;
-    `if m + n < p_256 then &(m + n) else &(m + n) - &p_256:real`] THEN
+    `if m + n < p_sm2 then &(m + n) else &(m + n) - &p_sm2:real`] THEN
   REPEAT CONJ_TAC THENL
    [CONV_TAC NUM_REDUCE_CONV THEN BOUNDER_TAC[];
-    REWRITE_TAC[p_256] THEN ARITH_TAC;
-    REWRITE_TAC[p_256] THEN ARITH_TAC;
+    REWRITE_TAC[p_sm2] THEN ARITH_TAC;
+    REWRITE_TAC[p_sm2] THEN ARITH_TAC;
     ALL_TAC;
     ASM_SIMP_TAC[MOD_ADD_CASES; GSYM NOT_LE; COND_SWAP] THEN
     COND_CASES_TAC THEN ASM_SIMP_TAC[GSYM REAL_OF_NUM_SUB] THEN
-    REWRITE_TAC[GSYM REAL_OF_NUM_CLAUSES; p_256] THEN REAL_ARITH_TAC] THEN
-  SUBGOAL_THEN `carry_s16 <=> (m + n) < p_256` (SUBST1_TAC o SYM) THENL
+    REWRITE_TAC[GSYM REAL_OF_NUM_CLAUSES; p_sm2] THEN REAL_ARITH_TAC] THEN
+  SUBGOAL_THEN `carry_s16 <=> (m + n) < p_sm2` (SUBST1_TAC o SYM) THENL
    [MATCH_MP_TAC FLAG_FROM_CARRY_LT THEN EXISTS_TAC `320` THEN
     MAP_EVERY EXPAND_TAC ["m"; "n"] THEN
     REWRITE_TAC[bignum_of_wordlist; MULT_CLAUSES; ADD_CLAUSES] THEN
-    REWRITE_TAC[GSYM REAL_OF_NUM_EQ; GSYM REAL_OF_NUM_ADD; p_256;
+    REWRITE_TAC[GSYM REAL_OF_NUM_EQ; GSYM REAL_OF_NUM_ADD; p_sm2;
                 GSYM REAL_OF_NUM_MUL; GSYM REAL_OF_NUM_POW] THEN
     ACCUMULATOR_ASSUM_LIST(MP_TAC o end_itlist CONJ o DECARRY_RULE) THEN
     DISCH_THEN(fun th -> REWRITE_TAC[th]) THEN
@@ -97,25 +97,25 @@ let BIGNUM_ADD_P256_CORRECT = time prove
     MAP_EVERY EXPAND_TAC ["m"; "n"] THEN
     ACCUMULATOR_POP_ASSUM_LIST(MP_TAC o end_itlist CONJ o DESUM_RULE) THEN
     REWRITE_TAC[WORD_AND_MASK; GSYM NOT_LE] THEN
-    REWRITE_TAC[GSYM REAL_OF_NUM_CLAUSES; bignum_of_wordlist; p_256] THEN
+    REWRITE_TAC[GSYM REAL_OF_NUM_CLAUSES; bignum_of_wordlist; p_sm2] THEN
     COND_CASES_TAC THEN ASM_REWRITE_TAC[BITVAL_CLAUSES] THEN
     CONV_TAC NUM_REDUCE_CONV THEN CONV_TAC WORD_REDUCE_CONV THEN
     DISCH_THEN(fun th -> REWRITE_TAC[th]) THEN REAL_INTEGER_TAC]);;
 
-let BIGNUM_ADD_P256_SUBROUTINE_CORRECT = time prove
+let BIGNUM_ADD_SM2_SUBROUTINE_CORRECT = time prove
  (`!z x y m n pc returnaddress.
         nonoverlapping (word pc,0x5c) (z,8 * 4)
         ==> ensures arm
-             (\s. aligned_bytes_loaded s (word pc) bignum_add_p256_mc /\
+             (\s. aligned_bytes_loaded s (word pc) bignum_add_sm2_mc /\
                   read PC s = word pc /\
                   read X30 s = returnaddress /\
                   C_ARGUMENTS [z; x; y] s /\
                   bignum_from_memory (x,4) s = m /\
                   bignum_from_memory (y,4) s = n)
              (\s. read PC s = returnaddress /\
-                  (m < p_256 /\ n < p_256
-                   ==> bignum_from_memory (z,4) s = (m + n) MOD p_256))
+                  (m < p_sm2 /\ n < p_sm2
+                   ==> bignum_from_memory (z,4) s = (m + n) MOD p_sm2))
           (MAYCHANGE [PC; X3; X4; X5; X6; X7; X8; X9; X10; X11] ,,
            MAYCHANGE SOME_FLAGS ,,
            MAYCHANGE [memory :> bignum(z,4)])`,
-  ARM_ADD_RETURN_NOSTACK_TAC BIGNUM_ADD_P256_EXEC BIGNUM_ADD_P256_CORRECT);;
+  ARM_ADD_RETURN_NOSTACK_TAC BIGNUM_ADD_SM2_EXEC BIGNUM_ADD_SM2_CORRECT);;
